Makefile
@@ -194,7 +194,7 @@ CLOSE=SmallstepClosed.v CompilerClosed.v
 
 CONCUR=MultiLibs.v CMulti.v AsmMulti.v \
        CallconvBig.v MultiSimBig.v \
-       HCompBig.v VCompBig.v
+       HCompBig.v InjpAccoComp.v VCompBig.v
 
 
 
